[kvs] Simplify proofs.

store/shared.v
@@ -7,7 +7,7 @@ From iris.base_logic.lib Require Import invariants.
 From iris.heap_lang Require Import notation proofmode.
 From iris.heap_lang.lib Require Import ticket_lock.
 From cryptis Require Import lib term gmeta nown.
-From cryptis Require Import cryptis primitives tactics role iso_dh conn rpc.
+From cryptis Require Import cryptis replica primitives tactics role iso_dh conn rpc.
 From cryptis.store Require Import alist db.
 
 Set Implicit Arguments.
@@ -36,13 +36,16 @@ Instance scs_repr : Repr server_client_state :=
   λ s, (scs_db s, scs_lock s)%V.
 
 Class storeGS Σ := StoreGS {
-  storeGS_db  : dbGS Σ;
+  storeGS_db : dbGS Σ;
+  storeGS_replica : replicaG Σ (list operation);
 }.
 
 Local Existing Instance storeGS_db.
+Local Existing Instance storeGS_replica.
 
 Definition storeΣ := #[
-  dbΣ
+  dbΣ;
+  replicaΣ (list operation)
 ].
 
 Global Instance subG_storeGS Σ : subG storeΣ Σ → storeGS Σ.
@@ -56,7 +59,8 @@ Notation iProp := (iProp Σ).
 Implicit Types (si : sess_info).
 Implicit Types (cs : Conn.state).
 Implicit Types (kI kR kS t : term) (ts : list term).
-Implicit Types db : gmap term term.
+Implicit Types (db : gmap term term).
+Implicit Types (o : operation) (os : list operation).
 Implicit Types accounts : gmap term server_client_state.
 Implicit Types n : nat.
 Implicit Types b : bool.
@@ -65,14 +69,24 @@ Implicit Types (failed : bool).
 
 Variable N : namespace.
 
+Definition db_client_ready kI kR db : iProp :=
+  ∃ os, ⌜db = DB.to_db os⌝ ∗
+        rep_main kI kR N os ∗ rep_current kI kR N [] os.
+
+Definition db_server_ready kI kR db : iProp :=
+  ∃ os, ⌜db = DB.to_db os⌝ ∗ rep_copy kI kR N [] os.
+
 Definition db_disconnected kI kR : iProp := ∃ db,
-  (Conn.failure kI kR ∨ DB.db_client_ready kI kR N db) ∗
+  (Conn.failure kI kR ∨ db_client_ready kI kR db) ∗
   DB.db_state kI kR N db.
 
-Definition db_connected kI kR cs : iProp := ∃ db,
-  RPC.client_connected kI kR cs ∗
-  (compromised_session Init cs ∨ DB.db_client_ready kI kR N db) ∗
+Definition db_connected' kI kR cs : iProp := ∃ db,
+  (compromised_session Init cs ∨ db_client_ready kI kR db) ∗
   DB.db_state kI kR N db.
+
+Definition db_connected kI kR cs : iProp :=
+  RPC.client_connected kI kR cs ∗
+  db_connected' kI kR cs.
 
 Lemma db_connected_ok kI kR cs :
   db_connected kI kR cs -∗
@@ -82,37 +96,37 @@ Lemma db_connected_ok kI kR cs :
   sign_key kR -∗
   ◇ □ ¬ compromised_session Init cs.
 Proof.
-iIntros "(% & conn & _ & _)".
+iIntros "(conn & _)".
 iApply (RPC.client_connected_ok with "conn").
 Qed.
 
-Definition rem_mapsto kI kR t1 t2 : iProp :=
+Definition db_mapsto kI kR t1 t2 : iProp :=
   DB.mapsto kI kR N t1 t2.
 
-Definition rem_free_at kI kR T : iProp :=
+Definition db_free_at kI kR T : iProp :=
   DB.free_at kI kR N T.
 
-Lemma rem_free_at_diff kI kR T1 T2 :
+Lemma db_free_at_diff kI kR T1 T2 :
   T1 ⊆ T2 →
-  rem_free_at kI kR T2 ⊣⊢ rem_free_at kI kR T1 ∗ rem_free_at kI kR (T2 ∖ T1).
+  db_free_at kI kR T2 ⊣⊢ db_free_at kI kR T1 ∗ db_free_at kI kR (T2 ∖ T1).
 Proof. iIntros "%sub". by iApply DB.free_at_diff. Qed.
 
 Lemma client_alloc kI kR E :
   ↑N.@"client".@kR ⊆ E →
   term_token kI E ={⊤}=∗
   db_disconnected kI kR ∗
-  rem_free_at kI kR ⊤ ∗
+  db_free_at kI kR ⊤ ∗
   term_token kI (E ∖ ↑N.@"client".@kR).
 Proof.
 iIntros "%sub kI_token".
 rewrite (term_token_difference _ _ _ sub).
 iDestruct "kI_token" as "[kI_token ?]". iFrame.
+iMod (rep_main_alloc (N := N) kI (kR := kR) [] with "kI_token")
+  as "(main & cur & kI_token)"; first solve_ndisj.
 iMod (DB.client_alloc _ (N := N) with "kI_token")
-  as "(ready & state & free & kI_token)".
+  as "(state & free & kI_token)".
 { solve_ndisj. }
-iModIntro. iSplitR "free".
-- by iFrame.
-- by iFrame.
+iModIntro. iFrame. iRight. iExists []. by iFrame.
 Qed.
 
 Definition public_db db : iProp :=
@@ -134,7 +148,7 @@ Qed.
 Definition server_db_connected' kI kR cs vdb : iProp := ∃ db,
   public_db db ∗
   SAList.is_alist vdb (repr <$> db) ∗
-  (compromised_session Resp cs ∨ DB.db_server_ready kI kR N db).
+  (compromised_session Resp cs ∨ db_server_ready kI kR db).
 
 Definition server_db_connected kI kR cs vdb : iProp :=
   RPC.server_connected kI kR cs ∗
@@ -146,7 +160,7 @@ Definition server_handler kI kR cs vdb h : iProp :=
 Definition server_db_disconnected kI kR vdb : iProp := ∃ db,
   public_db db ∗
   SAList.is_alist vdb (repr <$> db) ∗
-  (Conn.failure kI kR ∨ DB.db_server_ready kI kR N db).
+  (Conn.failure kI kR ∨ db_server_ready kI kR db).
 
 Lemma server_db_alloc kI kR vdb E :
   ↑N.@"server".@kI ⊆ E →
@@ -156,10 +170,10 @@ Lemma server_db_alloc kI kR vdb E :
   server_db_disconnected kI kR vdb.
 Proof.
 iIntros "%sub token vdb".
-iMod (DB.server_alloc with "token") as "(dis & token)"; eauto.
-iModIntro. iFrame "token". iExists ∅.
-iFrame.
-by rewrite /public_db big_sepM_empty.
+iMod (rep_copy_alloc with "token") as "[? rest]" => //.
+iFrame "rest". iModIntro. iExists ∅.
+iFrame. rewrite /public_db big_sepM_empty. iSplit => //.
+iRight. iExists []. by iFrame.
 Qed.
 
 Definition server ss : iProp := ∃ accounts E,
@@ -184,22 +198,168 @@ iPureIntro. move=> *. solve_ndisj.
 Qed.
 
 Definition store_call_pred kI kR si ts : iProp :=
-  ∃ t1 t2, ⌜ts = [t1; t2]⌝ ∗ DB.store_call kI kR N t1 t2.
+  ∃ t1 t2 os,
+    ⌜ts = [t1; t2]⌝ ∗
+    rep_update kI kR N [] os (os ++ [Store t1 t2]).
 
 Definition store_resp_pred kI kR si ts : iProp :=
-  DB.store_resp kI kR N.
+  ∃ os, rep_current kI kR N [] os.
 
-Definition load_call_pred kI kR si ts : iProp :=
-  ∃ t1, ⌜ts = [t1]⌝ ∗ DB.load_call kI kR N t1.
+(* MOVE *)
+Lemma to_db_app os o  :
+  DB.to_db (os ++ [o]) = DB.op_app (DB.to_db os) o.
+Proof. exact: foldl_app. Qed.
+(* /MOVE *)
 
-Definition load_resp_pred kI kR si ts : iProp :=
-  ∃ t2, ⌜ts = [t2]⌝ ∗ DB.load_resp kI kR N t2.
+Lemma store_call t2' kI kR cs t1 t2 :
+  let P := compromised_session Init cs in
+  db_connected' kI kR cs -∗
+  db_mapsto kI kR t1 t2 ==∗
+  (P ∨ store_call_pred kI kR cs [t1; t2']) ∗
+  db_mapsto kI kR t1 t2' ∗
+  ∀ ts, P ∨ store_resp_pred kI kR cs ts -∗ db_connected' kI kR cs.
+Proof.
+iIntros "% (%db & ready & own_db) own_frag".
+iMod (DB.db_state_update t2' with "own_db own_frag") as "[Hstate Hmapsto]".
+iFrame.
+iDestruct "ready" as "[#?|ready]".
+{ iModIntro. iSplitR; eauto.
+  iIntros "% _". iExists _. iFrame. eauto. }
+iDestruct "ready" as "(%os & -> & ready & cur)".
+iMod (rep_main_update (os ++ [Store t1 t2']) with "ready cur")
+  as "[ready cur]".
+iModIntro. iSplitL "cur".
+{ iRight. iExists _, _, _. by iFrame. }
+iIntros "%ts [#?|(%os' & cur)]".
+{ iExists _. iFrame. by eauto. }
+iPoseProof (rep_main_current with "ready cur") as "<-".
+iExists _. iFrame.
+iRight. iExists _. iFrame. by rewrite to_db_app.
+Qed.
+
+Lemma store_resp kI kR cs db t1 t2 :
+  let P := compromised_session Resp cs in
+  (P ∨ db_server_ready kI kR db) -∗
+  (P ∨ store_call_pred kI kR cs [t1; t2]) ==∗
+  (P ∨ db_server_ready kI kR (<[t1 := t2]>db)) ∗
+  (P ∨ store_resp_pred kI kR cs [TInt 0]).
+Proof.
+iIntros "% [#?|ready] [#?|call]"; try by iModIntro; iSplitL; eauto.
+iDestruct "ready" as "(%os & -> & ready)".
+iDestruct "call" as "(% & % & %os' & %e & upd)".
+case: e => <- <-.
+iMod (rep_copy_update with "ready upd") as "(<- & ready & cur)".
+iModIntro. iSplitL "ready"; iRight.
+- iExists _; iFrame. by rewrite to_db_app.
+- iExists _; iFrame.
+Qed.
 
 Definition create_call_pred kI kR si ts : iProp :=
-  ∃ t1 t2, ⌜ts = [t1; t2]⌝ ∗ DB.create_call kI kR N t1 t2.
+  ∃ t1 t2 os, ⌜ts = [t1; t2]⌝ ∗ ⌜DB.to_db os !! t1 = None⌝ ∗
+    rep_update kI kR N [] os (os ++ [Create t1 t2]).
 
 Definition create_resp_pred kI kR si ts : iProp :=
-  DB.create_resp kI kR N.
+  ∃ os, rep_current kI kR N [] os.
+
+Lemma create_call t1 t2 kI kR cs :
+  let P := compromised_session Init cs in
+  db_connected' kI kR cs -∗
+  db_free_at kI kR {[t1]} ==∗
+  (P ∨ create_call_pred kI kR cs [t1; t2]) ∗
+  db_mapsto kI kR t1 t2 ∗
+  ∀ ts, P ∨ create_resp_pred kI kR cs ts -∗
+        db_connected' kI kR cs.
+Proof.
+iIntros "% (%db & ready & state) free".
+iMod (DB.db_state_create t1 t2 with "state free") as "(%db_t1 & state & mapsto)".
+rewrite /= db_t1. iFrame.
+iDestruct "ready" as "[#?|(%os & -> & ready & cur)]".
+{ iModIntro; iSplitR; eauto.
+  iIntros "% _". iExists _. iFrame. eauto. }
+iMod (rep_main_update (os ++ [Create t1 t2]) with "ready cur")
+  as "[ready upd]".
+iModIntro. iSplitL "upd".
+{ iRight. iExists _, _, _. iFrame. by eauto. }
+iIntros "% [#?|(%os' & cur)]".
+{ iExists _. iFrame. by eauto. }
+iPoseProof (rep_main_current with "ready cur") as "<-".
+iExists _. iFrame. iRight.
+iExists _. iFrame. by rewrite to_db_app /= db_t1.
+Qed.
+
+Lemma create_resp kI kR cs db t1 t2 :
+  let P := compromised_session Resp cs in
+  (P ∨ db_server_ready kI kR db) -∗
+  (P ∨ create_call_pred kI kR cs [t1; t2]) ==∗
+  (P ∨ db_server_ready kI kR (<[t1 := t2]>db)) ∗
+  (P ∨ create_resp_pred kI kR cs [TInt 0]).
+Proof.
+iIntros "% [#?|ready] [#?|call]"; try by iModIntro; iSplitL; eauto.
+iDestruct "ready" as "(%os & -> & ready)".
+iDestruct "call" as "(% & % & %os' & %e & %db_t1 & upd)".
+case: e => <- <- in db_t1 *.
+iMod (rep_copy_update with "ready upd") as "(<- & ready & cur)".
+iModIntro. iSplitL "ready"; iRight.
+- iExists _; iFrame. by rewrite to_db_app /= db_t1.
+- iExists _; iFrame.
+Qed.
+
+Definition load_call_pred kI kR si ts : iProp :=
+  ∃ t1 t2 os, ⌜ts = [t1]⌝ ∗ ⌜DB.to_db os !! t1 = Some t2⌝ ∗
+              rep_update kI kR N [] os (os ++ [Load t1]).
+
+Definition load_resp_pred kI kR si ts : iProp :=
+  ∃ t1 t2 os, ⌜ts = [t2]⌝ ∗ ⌜DB.to_db os !! t1 = Some t2⌝ ∗
+              rep_current kI kR N [] (os ++ [Load t1]).
+
+Lemma load_call t1 t2 kI kR cs :
+  let P := compromised_session Init cs in
+  db_connected' kI kR cs -∗
+  db_mapsto kI kR t1 t2 ==∗
+  (P ∨ load_call_pred kI kR cs [t1]) ∗
+  db_mapsto kI kR t1 t2 ∗
+  ∀ ts, P ∨ load_resp_pred kI kR cs ts -∗
+        (P ∨ ⌜ts = [t2]⌝) ∗
+        db_connected' kI kR cs.
+Proof.
+iIntros "% (%db & ready & state) mapsto".
+iPoseProof (DB.db_state_mapsto with "state mapsto") as "%db_t1".
+iFrame.
+iDestruct "ready" as "[#?|(%os & -> & ready & cur)]".
+{ iModIntro. iSplitR; eauto.
+  iIntros "% _". iSplit; eauto. iExists _. iFrame. by eauto. }
+iMod (rep_main_update (os ++ [Load t1]) with "ready cur")
+  as "[ready cur]".
+iModIntro. iSplitR "ready state".
+{ iRight. iExists _, _, _. iFrame. by eauto. }
+iIntros "% [#?|(%t1' & %t2' & %os' & -> & %db_t1' & cur)]".
+{ iSplit; eauto. iFrame. by eauto. }
+iPoseProof (rep_main_current with "ready cur") as "%e".
+case: (app_inj_tail _ _ _ _ e) => [<- [<-]] in db_t1' *.
+rewrite db_t1' in db_t1. case: db_t1 => ->.
+iSplit; eauto. iExists _. iFrame.
+iRight. iExists _. iFrame. by rewrite to_db_app.
+Qed.
+
+Lemma load_resp kI kR cs db t1 :
+  let P := compromised_session Resp cs in
+  let t2 := default (TInt 0) (db !! t1) in
+  (P ∨ db_server_ready kI kR db) -∗
+  (P ∨ load_call_pred kI kR cs [t1]) ==∗
+  (P ∨ db_server_ready kI kR db) ∗
+  (P ∨ load_resp_pred kI kR cs [t2]).
+Proof.
+iIntros "%P /= [#?|ready] [#?|call]"; try by iModIntro; iSplitL; eauto.
+iDestruct "ready" as "(%os & -> & ready)".
+iDestruct "call" as "(%t1' & %t2 & %os' & %e & %db_t1 & upd)".
+case: e => <- in db_t1 *.
+iMod (rep_copy_update with "ready upd") as "(<- & ready & cur)".
+rewrite db_t1 /=. iModIntro.
+iSplitL "ready"; iRight.
+- iExists (os ++ [Load t1]). rewrite to_db_app /=.
+  by iFrame.
+- iExists _; iFrame. by eauto.
+Qed.
 
 Definition store_ctx : iProp :=
   RPC.rpc_pred N "store" store_call_pred store_resp_pred ∗
